% !TEX root = la.tex
\documentclass[10pt]{beamer}
\usepackage[utf8]{inputenc}

\usepackage{multirow,rotating}
\usepackage{color}
\usepackage{hyperref}
\usepackage{tikz-cd}
\usepackage{array}
\usepackage{siunitx}
\usepackage{mathtools,nccmath}%
\usepackage{etoolbox, xparse} 
\usetheme{CambridgeUS}
\usecolortheme{dolphin}

% set colors
\definecolor{myNewColorA}{RGB}{0, 24,150}
\definecolor{myNewColorB}{RGB}{0, 24,150}
\definecolor{myNewColorC}{RGB}{0, 24,150} % {130,138,143}
\setbeamercolor*{palette primary}{bg=myNewColorC}
\setbeamercolor*{palette secondary}{bg=myNewColorB, fg = white}
\setbeamercolor*{palette tertiary}{bg=myNewColorA, fg = white}
\setbeamercolor*{titlelike}{fg=myNewColorA}
\setbeamercolor*{title}{bg=myNewColorA, fg = white}
\setbeamercolor*{item}{fg=myNewColorA}
\setbeamercolor*{caption name}{fg=myNewColorA}
\usefonttheme{professionalfonts}
\usepackage{natbib}
\usepackage{hyperref}
%------------------------------------------------------------

\newcommand{\dfdh}{\frac{\partial f(\hat{h})}{\partial \hat{h_{i}}}}
\newcommand{\dgdh}{\frac{\partial g(\hat{h})}{\partial \hat{h_{i}}}}
\newcommand{\g}{\Sigma_{i}e^{h_{i}}}
\newcommand{\f}{\hat{e^{h_{t}}}}
\newcommand{\dghf}{\frac{\partial g(\hat{h})}{\partial h_{1}}}
\newcommand{\dghs}{\frac{\partial g(\hat{h})}{\partial h_{2}}}
\newcommand{\dght}{\frac{\partial g(\hat{h})}{\partial h_{3}}}
\newcommand{\dfhf}{\frac{\partial f(\hat{h})}{\partial h_{1}}}
\newcommand{\dfhs}{\frac{\partial f(\hat{h})}{\partial h_{2}}}
\newcommand{\dfht}{\frac{\partial f(\hat{h})}{\partial h_{3}}}

\setbeamerfont{title}{size=\large}
\setbeamerfont{subtitle}{size=\small}
\setbeamerfont{author}{size=\small}
\setbeamerfont{date}{size=\footnotesize}
\setbeamerfont{institute}{size=\footnotesize}
\title[RNN]{LSTM}

\begin{document}

%------------------------------------------------------------
\section{Optimiztion}

\begin{frame}{LSTM (Cell) Architecture}
    \begin{equation}
        o_{t} = \sigma(x_{t}*U^{o} + h_{t-1}*W^{o}), 
    \end{equation}
    \begin{equation}
        i_{t} = \sigma(x_{t}*U^{i} + h_{t-1}*W^{i}),
    \end{equation}
    \begin{equation}
        f_{t} = \sigma(x_{t}*U^{f} + h_{t-1}*W^{f}),
    \end{equation}
    \begin{equation}
        a_{t}  = \bar{c_{t}} = \tanh(x_{t}*U^{g} + h_{t-1}*W^{g}),
    \end{equation}
    \begin{equation}
        c_{t} = f_{t} * c_{t-1} + i_{t} * \bar{c_{t}},  
    \end{equation}
    \begin{equation}
        h_{t} = \tanh(c_{t}) * o_{t}.   
    \end{equation}
\end{frame}

\begin{frame}{Loss of the Layer through Time}
    Since we're operating (with $\partial$) on functions over the space $\mathbb{R}^{n}$ (this instance $n=3$) the composition operator 
    for $f, g$ is not multiplication any more, 
    i.e., we use the inner product of the vector space $\mathbb{R}^{3}$.
    \begin{align}
        p_{t} = \frac{\hat{e^{h}}}{\Sigma_{i}e^{h_{i}}} \text{, where } i\le dim(h_{t}) 
        \text{, and } t \le window_{time},\\
        \mathbf{L}(p_{t}) = -\ln(p_{t}),\\
        \frac{d}{dx}\left(\frac{f(x)}{g(x)}\right) = \frac{f'(x)g(x) - f(x)g'(x)}{[g(x)]^2},\\
        f(\hat{h}) = \f \text{, } \dfdh = e^{\hat{h_{i}}}\\
        g(\hat{h}) = \g \text{, } \dgdh = e^{h_{i}}\\
        g(\hat{h})^{2}   =  (e^{h_{1}}+e^{h_{2}}+e^{h_{3}})^{2}.
    \end{align}

\end{frame}

\begin{frame}
    \begin{align*}
        \dfhf g(\hat{h}) - f(x) \dghf &= \hat{e^{h_{1}}}\times \Sigma_{i}e^{h_{i}} - \hat{e^{h}}\cdot e^{h_{1}}\\
        &= [e^{h_{1}}, 0, 0]\times(e^{h_{1}}+e^{h_{2}}+e^{h_{3}}) -
        [e^{h_{1}}, e^{h_{2}}, e^{h_{3}}] \cdot [e^{h_{1}}, 0, 0]\\
        &= e^{2h_{1}} + e^{h_{1}}e^{h_{2}} + e^{h_{1}}e^{h_{3}} - e^{2h_{1}} \\
        &= e^{h_{1}}e^{h_{2}} + e^{h_{1}}e^{h_{3}}.
    \end{align*}
    \begin{align*}
        \frac{\partial p_{t}(\hat{h})}{\partial h_{1}} = 
        \frac{e^{h_{1}}e^{h_{2}} + e^{h_{1}}e^{h_{3}}}{(e^{h_{1}}+e^{h_{2}}+e^{h_{3}})^{2}},\\
        \frac{\partial \mathbf{L}(\hat{p_{t}})}{\partial h_{1}} = \frac{\partial \mathbf{L}(\hat{p_{t}})}{\partial \hat{p_{t}}}
        \frac{\partial p_{t}(\hat{h})}{\partial h_{1}} = -\frac{1}{p_{t}}
        \frac{e^{h_{1}}e^{h_{2}} + e^{h_{1}}e^{h_{3}}}{(e^{h_{1}}+e^{h_{2}}+e^{h_{3}})^{2}}.
    \end{align*}
\end{frame}

\begin{frame}
    \begin{align}
        \frac{\partial p_{t}(\hat{h})}{\partial h_{1}} = \frac{e^{h_{1}}e^{h_{2}} + e^{h_{1}}e^{h_{3}}}{(e^{h_{1}}+e^{h_{2}}+e^{h_{3}})^{2}},\\
        \frac{\partial p_{t}(\hat{h})}{\partial h_{2}} = \frac{e^{h_{2}}e^{h_{1}} + e^{h_{2}}e^{h_{3}}}{(e^{h_{1}}+e^{h_{2}}+e^{h_{3}})^{2}},\\
        \frac{\partial p_{t}(\hat{h})}{\partial h_{3}} = \frac{e^{h_{3}}e^{h_{1}} + e^{h_{3}}e^{h_{2}}}{(e^{h_{1}}+e^{h_{2}}+e^{h_{3}})^{2}}.
    \end{align}
\end{frame}

\end{document}


